Given an array of integers ```A``` and let n to be its length.

Assume ```Bk``` to be an array obtained by rotating the array ```A``` k positions clock-wise, we define a "rotation function" ```F``` on ```A``` as follow:

```
F(k) = 0 * Bk[0] + 1 * Bk[1] + ... + (n-1) * Bk[n-1]
```


Calculate the maximum value of F(0), F(1), ..., F(n-1).

__Note:__ n is guaranteed to be less than 105.

#### Example:

```
A = [4, 3, 2, 6]

F(0) = (0 * 4) + (1 * 3) + (2 * 2) + (3 * 6) = 0 + 3 + 4 + 18 = 25
F(1) = (0 * 6) + (1 * 4) + (2 * 3) + (3 * 2) = 0 + 4 + 6 + 6 = 16
F(2) = (0 * 2) + (1 * 6) + (2 * 4) + (3 * 3) = 0 + 6 + 8 + 9 = 23
F(3) = (0 * 3) + (1 * 2) + (2 * 6) + (3 * 4) = 0 + 2 + 12 + 12 = 26

So the maximum value of F(0), F(1), F(2), F(3) is F(3) = 26.
```

# Solution

Look at the example given above:

* from ```F(0) = (0 * 4) + (1 * 3) + (2 * 2) + (3 * 6)``` to ```F(1) = (0 * 6) + (1 * 4) + (2 * 3) + (3 * 2)```, we can see that ```F(1) = F(0) + (4 + 3 + 2 + 6) - (4 * 6) = F(0) + sum - (4 * 6)```.
* from ```F(1) = (0 * 6) + (1 * 4) + (2 * 3) + (3 * 2)``` to ```F(2) = (0 * 2) + (1 * 6) + (2 * 4) + (3 * 3)```, we can see that ```F(2) = F(1) + (6 + 4 + 3 + 2) - (4 * 2) = F(1) + sum - (4 * 2)```.
* from ```F(2) = (0 * 2) + (1 * 6) + (2 * 4) + (3 * 3)``` to ```F(3) = (0 * 3) + (1 * 2) + (2 * 6) + (3 * 4)```, we can see that ```F(3) = F(2) + (2 + 6 + 4 + 3) - (4 * 3) = F(2) + sum - (4 * 3)```.

These observation give us enough reason to believe that we may come up with a general law to migrate from ```F(i - 1)``` to ```f(i)``` through induction. And that general raw is ```F(i) = F(i - 1) + sum - size_of_A * A[size_of_A - i]```, since here ```i``` basically means the i-th clock-wise rotation. It can also be expressed as  ``F(k) = F(k - 1) + sum - size_of_A * A[size_of_A - k]```, which is the same.

Right now what left is only a rigorous proof:

```
F(k) = 0 * Bk[0-k] + 1 * Bk[1-k] + … + (n-1) * Bk[n-1-k]
F(k+1) = 0 * Bk[n-(k+1)] + 1 * Bk[1-(k+1)] + … + (n-2) * Bk[n-1-(k+1)]
= 0 * Bk[n- 1 - k] + 1 * Bk[0-k] + … + (n-2) * Bk[n-2-k]
= 0 * Bk[0-k] + 1 * Bk[1-k] + … + (n-1) * Bk[n-1-k] + sum - n *Bk[n-(k+1)]
Note: Bk[n- 1 - k] == Bk[n-(k+1)]
```

```cpp
class Solution {
public:
    int maxRotateFunction(vector<int>& A) {
        int sum = std::accumulate(A.begin(), A.end(), 0);
        const int size(A.size());
        int val(0);
        for (int i = 0; i < size; ++i) {
            val += i * A[i];
        }
        
        int reval(val);
        for (int i = 1; i < size; ++i) {
            val = val + sum - size * A[size - i];
            reval = std::max(reval, val);
        }
        
        return reval;
    }
};
```
